PropositionalLogic/Syntax.v
@@ -4,22 +4,13 @@ Require Export Coq.Relations.Relation_Definitions.
 Require Export Coq.Classes.RelationClasses.
 Require Import Logic.LogicBase.
 
-Class PropositionalLanguage: Type := {
-  expr: Type;
+Class PropositionalLanguage (L: Language) {nL: NormalLanguage L}: Type := {
   andp : expr -> expr -> expr;
   orp : expr -> expr -> expr;
-  imp : expr -> expr -> expr;
   iffp : expr -> expr -> expr;
   negp : expr -> expr;
-  truep : expr;
-  falsep : expr
+  truep : expr
 }.
-
-Instance PropositionalLanguage_Language (L: PropositionalLanguage): Language :=
-  Build_Language expr.
-
-Instance PropositionalLanguage__nLanguage (L: PropositionalLanguage):  NormalLanguage _ :=
-  Build_NormalLanguage (PropositionalLanguage_Language L) falsep imp.
 
 Notation "x && y" := (andp x y) (at level 40, left associativity) : PropositionalLogic.
 Notation "x || y" := (orp x y) (at level 50, left associativity) : PropositionalLogic.
@@ -30,6 +21,51 @@ Notation "'FF'" := falsep : PropositionalLogic.
 Notation "'TT'" := truep : PropositionalLogic.
 
 Local Open Scope PropositionalLogic.
+
+Inductive prop_congr {L: Language} {nL: NormalLanguage L} {pL: PropositionalLanguage L} {atomic_reduce: relation expr}: relation expr :=
+| atomic_step: forall x y, atomic_reduce x y -> prop_congr x y
+| andp_congr: forall x1 x2 y1 y2, prop_congr x1 y1 -> prop_congr x2 y2 -> prop_congr (x1 && x2) (y1 && y2)
+| orp_congr: forall x1 x2 y1 y2, prop_congr x1 y1 -> prop_congr x2 y2 -> prop_congr (x1 || x2) (y1 || y2)
+| imp_congr: forall x1 x2 y1 y2, prop_congr x1 y1 -> prop_congr x2 y2 -> prop_congr (x1 --> x2) (y1 --> y2)
+| iffp_congr: forall x1 x2 y1 y2, prop_congr x1 y1 -> prop_congr x2 y2 -> prop_congr (x1 <--> x2) (y1 <--> y2)
+| negp_congr: forall x y, prop_congr x y -> prop_congr (~~ x) (~~ y)
+.
+
+(* Locate clos_refl_trans. *)
+
+Arguments prop_congr {L} {nL} {pL} atomic_reduce _ _.
+
+Module ImpNegAsPrime.
+
+Inductive atomic_reduce {L: Language} {nL: NormalLanguage L} {pL: PropositionalLanguage L}: expr -> expr -> Prop :=
+| andp_reduce: forall x y, atomic_reduce (x && y) (~~ (x --> ~~ y))
+| orp_reduce: forall x y, atomic_reduce (x || y) (~~ x --> y)
+.
+
+End ImpNegAsPrime.
+
+Module ImpAndOrAsPrime.
+
+Inductive atomic_reduce {L: Language} {nL: NormalLanguage L} {pL: PropositionalLanguage L}: expr -> expr -> Prop :=
+| negp_reduce: forall x, atomic_reduce (~~ x) (x --> FF)
+.
+
+End ImpAndOrAsPrime.
+
+Module ReduceIff.
+
+Inductive atomic_reduce {L: Language} {nL: NormalLanguage L} {pL: PropositionalLanguage L}: expr -> expr -> Prop :=
+| iff_reduce: forall x y, atomic_reduce (x <--> y) ((x --> y) && (y --> x)).
+
+End ReduceIff.
+
+Module ReduceTrueFalse.
+
+Inductive atomic_reduce {L: Language} {nL: NormalLanguage L} {pL: PropositionalLanguage L}: expr -> expr -> Prop :=
+| falsep_reduce: atomic_reduce FF (~~ TT)
+| truep_reduce: forall x, atomic_reduce TT (x --> x).
+
+End ReduceTrueFalse.
 
 Module PropositionalLanguage.
 
@@ -45,54 +81,9 @@ Inductive expr {Var: Type}: Type :=
 
 Implicit Arguments expr.
 
-Instance PropositionalLanguage (Var: Type): PropositionalLanguage :=
-  Build_PropositionalLanguage (expr Var) andp orp imp iffp negp truep falsep.
+Instance L (Var: Type): Language := Build_Language (expr Var).
+Instance nL (Var: Type): NormalLanguage (L Var) := Build_NormalLanguage (L Var) falsep imp.
+Instance pL (Var: Type): PropositionalLanguage (L Var) := Build_PropositionalLanguage (L Var) (nL Var) andp orp iffp negp truep.
 
 End PropositionalLanguage.
-
-Inductive prop_congr {L: PropositionalLanguage} {atomic_reduce: relation expr}: relation expr :=
-| atomic_step: forall x y, atomic_reduce x y -> prop_congr x y
-| andp_congr: forall x1 x2 y1 y2, prop_congr x1 y1 -> prop_congr x2 y2 -> prop_congr (x1 && x2) (y1 && y2)
-| orp_congr: forall x1 x2 y1 y2, prop_congr x1 y1 -> prop_congr x2 y2 -> prop_congr (x1 || x2) (y1 || y2)
-| imp_congr: forall x1 x2 y1 y2, prop_congr x1 y1 -> prop_congr x2 y2 -> prop_congr (x1 --> x2) (y1 --> y2)
-| iffp_congr: forall x1 x2 y1 y2, prop_congr x1 y1 -> prop_congr x2 y2 -> prop_congr (x1 <--> x2) (y1 <--> y2)
-| negp_congr: forall x y, prop_congr x y -> prop_congr (~~ x) (~~ y)
-.
-
-(* Locate clos_refl_trans. *)
-
-Arguments prop_congr {L} atomic_reduce _ _.
-
-Module ImpNegAsPrime.
-
-Inductive atomic_reduce {L: PropositionalLanguage}: expr -> expr -> Prop :=
-| andp_reduce: forall x y, atomic_reduce (x && y) (~~ (x --> ~~ y))
-| orp_reduce: forall x y, atomic_reduce (x || y) (~~ x --> y)
-.
-
-End ImpNegAsPrime.
-
-Module ImpAndOrAsPrime.
-
-Inductive atomic_reduce {L: PropositionalLanguage}: expr -> expr -> Prop :=
-| negp_reduce: forall x, atomic_reduce (~~ x) (x --> FF)
-.
-
-End ImpAndOrAsPrime.
-
-Module ReduceIff.
-
-Inductive atomic_reduce {L: PropositionalLanguage}: expr -> expr -> Prop :=
-| iff_reduce: forall x y, atomic_reduce (x <--> y) ((x --> y) && (y --> x)).
-
-End ReduceIff.
-
-Module ReduceTrueFalse.
-
-Inductive atomic_reduce {L: PropositionalLanguage}: expr -> expr -> Prop :=
-| falsep_reduce: atomic_reduce FF (~~ TT)
-| truep_reduce: forall x, atomic_reduce TT (x --> x).
-
-End ReduceTrueFalse.
-
 
