PropositionalLogic/TrivialSemantics.v
@@ -1,0 +1,38 @@
+Require Import Logic.LogicBase.
+Require Import Logic.PropositionalLogic.Syntax.
+
+Module TrivialSemantics.
+
+Import PropositionalLanguage.
+
+Definition model (Var: Type): Type := Var -> Prop.
+
+Definition sem_imp {Var: Type} (X: Ensemble (model Var)) (Y: Ensemble (model Var)): Ensemble (model Var) :=
+  fun m => X m -> Y m.
+
+Definition sem_neg {Var: Type} (X: Ensemble (model Var)): Ensemble (model Var) :=
+  fun m => ~ X m.
+
+Definition sem_and {Var: Type} (X: Ensemble (model Var)) (Y: Ensemble (model Var)): Ensemble (model Var) :=
+  sem_neg (sem_imp (sem_neg X) Y).
+
+Definition sem_or {Var: Type} (X: Ensemble (model Var)) (Y: Ensemble (model Var)): Ensemble (model Var) :=
+  sem_neg (sem_imp (sem_neg X) Y).
+
+Definition sem_iff {Var: Type} (X: Ensemble (model Var)) (Y: Ensemble (model Var)): Ensemble (model Var) :=
+  sem_and (sem_imp X Y) (sem_imp Y X).
+
+Fixpoint denotation {Var: Type} (x: expr Var): Ensemble (model Var) :=
+  match x with
+  | andp y z => sem_and (denotation y) (denotation z)
+  | orp y z => sem_or (denotation y) (denotation z)
+  | imp y z => sem_imp (denotation y) (denotation z)
+  | iffp y z => sem_iff (denotation y) (denotation z)
+  | negp y => sem_neg (denotation y)
+  | truep => fun _ => True
+  | falsep => fun _ => False
+  | varp p => fun m => m p
+  end.
+
+Instance TrivialModel (Var: Type): Semantics (PropositionalLanguage.L Var) :=
+  Build_Semantics (PropositionalLanguage.L Var) (model Var) (fun m x => denotation x m).
